{
 "cells": [
  {
   "cell_type": "markdown",
   "metadata": {},
   "source": [
    "#### Two definitions\n",
    "\n",
    "Imagine two vectors $ A =[a_x,a_y]$ and $ B = [b_x,b_y]  $\n",
    "\n",
    "The dot product is given by following two definitions:  \n",
    "\n",
    "1. $ a_xb_x + a_yb_y $\n",
    "2. $|A||B|cos \\theta $  \n",
    "\n",
    "#### How these two definitions are equivalent?  \n",
    "\n",
    "One proof based on components is here : https://math.stackexchange.com/a/2629588\n",
    "\n",
    "##### Alternatively:\n",
    "\n",
    "![dot_product_equivalence](dot_product_equivalence_2.png)\n",
    "\n",
    "(Source: https://www.geogebra.org/calculator/artwuzxc)\n",
    "\n",
    "Imagine a plane with x and y axis. Let's say vector A makes angle of $\\theta_1$ with the x-axis, and vector B makes angle of $\\theta_2 > \\theta_1$ with x-axis, and let $\\theta$ be the angle between the two vectors.\n",
    "\n",
    "Therefore,\n",
    "\n",
    "$  a_x = |A|cos\\theta_1$  \n",
    "$  a_y = |A|sin\\theta_1$  \n",
    "$  b_x = |B|cos\\theta_2$  \n",
    "$  b_y = |B|sin\\theta_2$  \n",
    "$ \\theta = \\theta_2 - \\theta_1 $  \n",
    "\n",
    "$ a_xb_x + a_yb_y = |A|cos\\theta_1 |B|cos\\theta_2 + |A|sin\\theta_1|B|sin\\theta_2$  \n",
    "\n",
    "$ = |A||B|cos\\theta_1cos\\theta_2 + |A||B|sin\\theta_1sin\\theta_2 $ \n",
    "\n",
    "$ = |A||B|(cos\\theta_1cos\\theta_2 + sin\\theta_1sin\\theta_2) $ \n",
    "\n",
    "![cos_a_minus_b](cos_a_minus_b.png)\n",
    "\n",
    "In the above figure,$\\theta_1$ and $\\theta_2$ are any general angles (not to be correlated with the angles in the first figure).  $\\angle AFE $ and $\\angle AEB $ are chosen to be right angles.\n",
    "\n",
    "\n",
    "$\\angle EAB + \\angle ABD + \\angle DBE = 90^o$  \n",
    "\n",
    "$\\theta_2 - \\theta_1 + \\angle ABD + \\angle DBE = 90^o$\n",
    "\n",
    "$\\theta_2 + \\angle ABD - \\theta_1 + \\angle DBE = 90^o$$\\tag 1$  \n",
    "\n",
    "\n",
    "$\\angle CAE + \\angle EAB + \\angle ABD = 90^o$  \n",
    "\n",
    "$ \\theta_1 + (\\theta_2 - \\theta_1) + \\angle ABD =  90^o$  \n",
    "\n",
    "$ \\theta_2 + \\angle ABD =  90^o$$\\tag 2$  \n",
    "\n",
    "\n",
    "Substituting (2) in (1)  \n",
    "\n",
    "$90^o - \\theta_1 + \\angle DBE = 90^o$   \n",
    "\n",
    "$ - \\theta_1 + \\angle DBE = 0$   \n",
    "\n",
    "$ \\angle DBE = \\theta_1 = \\angle CAE $$\\tag 3$   \n",
    "\n",
    "Therefore,  \n",
    "\n",
    "$tan\\theta_1 = \\frac{EF}{AF} = \\frac{DE}{BD} = \\frac{CF}{BD} $  \n",
    "\n",
    "$ BD*EF = AF*CF $$\\tag 4$\n",
    "\n",
    "\n",
    "\n",
    "\n",
    "$ cos\\theta_1cos\\theta_2 + sin\\theta_1sin\\theta_2$  \n",
    "\n",
    "$ = \\frac{AC}{AB} \\frac{AF}{AE} + \\frac{BC}{AB} \\frac{EF}{AE}$  \n",
    "\n",
    "$ = \\frac{AC*AF+BC*EF}{AB*AE}$  \n",
    "\n",
    "$ = \\frac{(AF-CF)AF+(BD+EF)EF}{AB*AE}$  \n",
    "\n",
    "$ = \\frac{AF^2 - AF*CF + BD*EF +EF^2}{AB*AE}$  \n",
    "\n",
    "$ = \\frac{AF^2 +EF^2 + BD*EF - AF*CF }{AB*AE}$  \n",
    "\n",
    "$ = \\frac{AE^2 + BD*EF - AF*CF }{AB*AE}$  \n",
    "\n",
    "$ = \\frac{AE^2 + 0 }{AB*AE}$$\\tag{from 4}$  \n",
    "\n",
    "$ = \\frac{AE}{AB}$  \n",
    "\n",
    "$ = cos(\\angle BAE)$  \n",
    "\n",
    "$ = cos(\\theta_2 - \\theta_1)$  \n",
    "\n",
    "$ = cos\\theta $  \n",
    "\n",
    "Therefore in general:  \n",
    "\n",
    "$ cos\\theta_1cos\\theta_2 + sin\\theta_1sin\\theta_2 = cos(\\theta_2 - \\theta_1) = cos\\theta$  \n",
    "\n",
    "Now returning to our original equation:  \n",
    "\n",
    "$ a_xb_x + a_yb_y = |A||B|(cos\\theta_1cos\\theta_2 + sin\\theta_1sin\\theta_2)$  \n",
    "\n",
    "$ = |A||B|cos(\\theta_2 - \\theta_1) $ \n",
    "\n",
    "$ = |A||B|cos(\\theta) $ \n",
    "\n",
    "\n",
    "#### Alternate Proof of : $ cos(\\theta_2 - \\theta_1) $  \n",
    "\n",
    "\n",
    "$cos\\theta$ and $sin\\theta$ are basically respectively x and y co-ordinates of the intersection of the radius at angle $\\theta$ with x-axis and the unit circle. When the angle is $-\\theta$, x-co-ordinate remains same and positive while the y-co-ordinate becomes negative.  \n",
    "\n",
    "$ \\therefore x = cos(-\\theta) = cos(\\theta)$ and $ y = sin(-\\theta)=-sin(\\theta) $  \n",
    "\n",
    "Proof of $cos(\\theta_1 + \\theta_2)$: https://www.youtube.com/watch?v=V3-xCPDzQ1Q  \n",
    "\n",
    "\n",
    "$ cos(\\theta) = cos(\\theta_2 - \\theta_1) $  \n",
    "\n",
    "$ = cos(\\theta_2 + (-\\theta_1)) $  \n",
    "\n",
    "$ = cos\\theta_2 cos(-\\theta_1) - sin(\\theta_2)sin(-\\theta_1)$  \n",
    "\n",
    "$ = cos\\theta_2 cos\\theta_1 + sin\\theta_2sin\\theta_1$  \n",
    "\n",
    "\n",
    "\n",
    "\n",
    "\n",
    "\n",
    "\n",
    "\n",
    "\n"
   ]
  },
  {
   "cell_type": "code",
   "execution_count": null,
   "metadata": {},
   "outputs": [],
   "source": []
  },
  {
   "cell_type": "code",
   "execution_count": null,
   "metadata": {},
   "outputs": [],
   "source": []
  }
 ],
 "metadata": {
  "kernelspec": {
   "display_name": "Python 3",
   "language": "python",
   "name": "python3"
  },
  "language_info": {
   "codemirror_mode": {
    "name": "ipython",
    "version": 3
   },
   "file_extension": ".py",
   "mimetype": "text/x-python",
   "name": "python",
   "nbconvert_exporter": "python",
   "pygments_lexer": "ipython3",
   "version": "3.6.4"
  }
 },
 "nbformat": 4,
 "nbformat_minor": 5
}
