{
 "cells": [
  {
   "cell_type": "markdown",
   "id": "6643d37e",
   "metadata": {},
   "source": [
    "#### Chain Rule\n",
    "\n",
    "\n",
    "\n",
    "$ \\frac{dy}{dx} $ is the derivative or instantaneous slope at a given point.  \n",
    "\n",
    "$ \\frac{d}{dx} x^2  = 2x$$\\tag{1.1}$  \n",
    "It means when x changes by dx, y changes by 2x.dx  \n",
    "\n",
    "$ dy = 2x dx$  \n",
    "\n",
    "\n",
    "\n",
    "Consider following functions:  \n",
    "\n",
    "$ y = f(x) $  \n",
    "$ z = g(y) $  \n",
    "\n",
    "If we fix the value of x to a constant c, values of y and z above will also be fixed to the constants f(c) and g(f(c)) respectively.  \n",
    "\n",
    "\n",
    "When we fix x = c, $\\frac{dy}{dx}$, which is also a function of x, $f'(x) =\\frac{dy}{dx}$ is also fixed. For example, in (1) above, $f'(x) =\\frac{dy}{dx} = 2x = 2c$$\\tag{1.2}$  \n",
    "\n",
    "$dy = f'(x)dx = f'(c)dx$  \n",
    "\n",
    "Means for a fixed value of x=c, dy is only function of dx.  \n",
    "\n",
    "We can have same argument for dz, for a fixed value of y, say $c_1 = f(c)$ (which we got by fixing x=c first),  \n",
    "\n",
    "dz is only function of dy (and transitively dx because dy is function of dx)  \n",
    "\n",
    "Now consider following figure:(https://www.geogebra.org/m/k55rxwde)  \n",
    "\n",
    "![chain_rule](chainrule.png)\n",
    "\n",
    "(Note that the sharing of dy(segment BD) between the two right angle triangle illustrates the chain-effect of dx on dz)\n",
    "(Also note that dx,dy and dz are almost 0 (lim -> 0), but for illustration we have shown their concrete scaled values in above figure)\n",
    "\n",
    "Here  \n",
    "\n",
    "slope of line AB = m1 = $\\frac{dy}{dx}$  \n",
    "\n",
    "$dy = m1*dx$$\\tag{1.3}$  \n",
    "\n",
    "slope of line BC = m2 = $\\frac{dz}{dy}$  \n",
    "\n",
    "$dz = m2*dy$$\\tag{1.4}$  \n",
    "\n",
    "Note that m1 and m2 are constants(fixed) as we discussed in (1.2)  \n",
    "\n",
    "$dz = m2*m1*dx $$\\tag {from 1.3 and 1.4 above}$  \n",
    "\n",
    "$\\frac{dz}{dx} = m2*m1$  \n",
    "\n",
    "Note segments DC and DE are exactly same in above figure, therefore   \n",
    "\n",
    "slope of line AE = $\\frac{dz}{dx} = m2*m1 = \\frac{dz}{dy}\\frac{dy}{dx}$  \n",
    "\n",
    "\n",
    "\n",
    "\n",
    "\n",
    "\n",
    "\n",
    "#### An example\n",
    "\n",
    "Now consider following relations  \n",
    "\n",
    "$ x = w^2 $  \n",
    "$ y = x^3 $  \n",
    "$ z = 5y  $  \n",
    "\n",
    "$ \\frac{dx}{dw} = 2w $  \n",
    "$ \\frac{dy}{dx} = 3x^2 $  \n",
    "$ \\frac{dz}{dy} = 5 $  \n",
    "\n",
    "$ dx = 2w dw $  \n",
    "$ dy = 3x^2 dx $  \n",
    "$ dz = 5 dy $  \n",
    "\n",
    "$ dz = 5 *3x^2 dx $  \n",
    "$ dz = 5 *3x^2 * 2w dw $  \n",
    "\n",
    "$ \\therefore$  \n",
    "\n",
    "$ \\frac{dz}{dx} = 5 *3x^2 = \\frac{dz}{dy}\\frac{dy}{dx} $  \n",
    "\n",
    "$ \\frac{dz}{dw} = 5 *3x^2 * 2w = \\frac{dz}{dy}\\frac{dy}{dx}\\frac{dx}{dw} $  \n",
    "\n",
    "Also  \n",
    "\n",
    "$ \\frac{dz}{dw} = \\frac{dz}{dy}\\frac{dy}{dw}$  \n",
    "\n",
    "\n",
    "##### Important note: If we know a derivative $\\frac{dy}{dw}$ and we know the relation between z and y, we can calculate $\\frac{dz}{dw} $ using chain rule  \n",
    "\n",
    "#### In General:\n",
    "\n",
    "$ z = g(y) $  \n",
    "$ y = f(x) $  \n",
    "\n",
    "$ \\frac{dz}{dy} = g'(y) $  \n",
    "\n",
    "$ dz = g'(y) dy $$\\tag {2.1}$  \n",
    "\n",
    "$ \\frac{dy}{dx} = f'(x) $  \n",
    "\n",
    "$ dy = f'(x)dx $$\\tag {2.2}$    \n",
    "\n",
    "$ dz = g'(y)f'(x)dx $$\\tag {from (2.1) and (2.2)}$    \n",
    "\n",
    "$ \\frac{dz}{dx} = g'(y)f'(x) $  \n",
    "\n",
    "$ \\frac{dz}{dx} = \\frac{dz}{dy} \\frac{dy}{dx} $  \n",
    "\n",
    "\n",
    "The chain can be very long, if we know the derivative of last term to y, and if we know relation between x and y, we can get derivatove of last term to x.\n",
    "\n",
    "$ \\frac{dx_1}{dx_5} = \\frac{dx_1}{dx_4}\\frac{dx_4}{dx_5} $  \n",
    "\n",
    "$ \\frac{dx_1}{dx_4} = \\frac{dx_1}{dx_3}\\frac{dx_3}{dx_4} $ \n",
    "\n",
    "and so on...\n",
    "\n",
    "\n",
    "\n",
    "\n",
    "\n",
    "\n",
    "\n",
    "\n",
    "\n",
    "\n",
    "\n",
    "\n"
   ]
  },
  {
   "cell_type": "code",
   "execution_count": null,
   "id": "ab08a6e9",
   "metadata": {},
   "outputs": [],
   "source": []
  },
  {
   "cell_type": "code",
   "execution_count": null,
   "id": "42c6f85e",
   "metadata": {},
   "outputs": [],
   "source": []
  },
  {
   "cell_type": "code",
   "execution_count": null,
   "id": "fbfedcf9",
   "metadata": {},
   "outputs": [],
   "source": []
  }
 ],
 "metadata": {
  "kernelspec": {
   "display_name": "Python 3",
   "language": "python",
   "name": "python3"
  },
  "language_info": {
   "codemirror_mode": {
    "name": "ipython",
    "version": 3
   },
   "file_extension": ".py",
   "mimetype": "text/x-python",
   "name": "python",
   "nbconvert_exporter": "python",
   "pygments_lexer": "ipython3",
   "version": "3.8.1"
  }
 },
 "nbformat": 4,
 "nbformat_minor": 5
}
