#### Sum of exponents

$ x^a * x^b = (x * x * ... * x) * (x * x * ... x) $   
 = (x multiplied to itself a times) * (x multiplied to itself b times)  
 = (x multiplied to itself a+b times )  
$ = x^{(a+b)} $  

$ x^3 * x ^4 $  
$ = (x * x * x) * (x * x * x * x) $   
$ = x * x * x * x * x * x * x $  
$ = x^7 $  
$ = x^{(3+4)} $   

#### Exponent of exponent expression

$ (x^a)^3 = (x^a)*(x^a)*(x^a) $  
$ = x^{a+a+a} $  
$ = x^{3a} $  

In general:  

$ (x^a)^b = x^{ab} $  

#### Negative exponents  

$ x^2 = \frac{x^3}{x} $  

$ x^1 = \frac{x^2}{x} $ 

$ x^0 = \frac{x^1}{x} = 1 $  

$ x^{-1} = \frac{x^0}{x} = \frac{1}{x} $  

$ x^{-2} = \frac{x^{-1}}{x} = \frac{\frac{1}{x}}{x} = \frac{1}{x^2} $  

#### Fractional exponents

$ x^{\frac{1}{2}} * x^{\frac{1}{2}} = x^{(\frac{1}{2}+\frac{1}{2})} = x^1 $  

$ x = x^1 = x^{\frac{1}{2}} * x^{\frac{1}{2}} $  

$ x = (x^{\frac{1}{2}})^2 $  

$ x^{\frac{1}{2}} = \sqrt{x} $  

In general:

$ (x^{\frac{1}{a}})^a $  

$ = x^{\frac{1}{a}} * x^{\frac{1}{a}} * ... * x^{\frac{1}{a}} $   ... a times  

$ = x^{\frac{1+1+1+ ... + 1 a times}{a}} $  

$ = x^{\frac{1}{1}} $  

$ = x $  

$ (x^{\frac{1}{a}})^a = x $  

$  (x^{\frac{1}{a}}) = \sqrt[a]x $  



#### Basic logarithms
https://www.mathsisfun.com/algebra/logarithms.html 

$ log_{10}(10) = 1 $  

$ log_{10}(100) = 2 $  

$ log_{10}(10^n) = n $  

$ log_{10}(10^0) = log_{10}(1) = 0 $  

$ log_{10}(10^{-1}) = -1 $  

$ log_{10}(\sqrt{10}) = log_{10}(10^{\frac{1}{2}}) = \frac{1}{2} $ 

#### Log of multiplications

$ log_b (x) = p $ ...1  
$ log_b (y) = q $ ...2

by definition 

$ b^p = x $  
$ b^q = y $  

$ log_b (x * y) $  

$ = log_b (b^p * b^q) $  

$ = log_b (b ^{p+q}) $  

$ = p + q $  

$ = log_b (x) + log_b (y)  $  ...from 1 and 2 above

#### Log of exponents

$ log_b (m^n) = log_b(m * m * ... * m) $ ... n times  

$ = log_b(m) + log_b(m) + log_b(m) + ... + log_b(m) $ ... n times  

$ = n * log_b(m) $  

#### Log of negative exponenets

$ log_b (x^{-1}) = p $  ... 1

by definition 

$ b^p = x^{-1} $  

$ b^p = \frac{1}{x} $  

$ x = \frac{1}{b^p} $  

$ x = b^{-p} $  

$ log_b(x) = log(b^{-p}) $  

$ log_b(x) = -p $  

$ p = -log_b(x) $  

$ log_b (x^{-1}) = -log_b(x) $  ... from 1
















 






