$ ax^2+bx+c $ 

$ =a\cdot\left(x^2+\frac {b}{a}x+\frac{c}{a} \right)$ 

$ =a\cdot\left(x^2+\frac {2b}{2a}x+\frac{c}{a} \right)$ 

$ =a\cdot\left(x^2+2\frac {b}{2a}x+\frac{c}{a} \right)$ 

$ =a\cdot\left(x^2+2\frac {b}{2a}x+ \frac{b^2}{4a^2}-\frac{b^2}{4a^2}+ \frac{c}{a} \right)$ 

$ =a\cdot\left(\left(x^2+2\frac {b}{2a}x+ \frac{b^2}{4a^2}\right)-\frac{b^2}{4a^2}+ \frac{c}{a} \right)$ 

$ =a\cdot\left(\left(x+\frac {b}{2a}\right)^2-\frac{b^2}{4a^2}+ \frac{c}{a} \right)$ 

$ =a\cdot\left(x+\frac b{2a}\right)^2-\frac{b^2}{4a}+c $  

$ =a\cdot\left(x+\frac b{2a}\right)^2-\frac{b^2-4ac}{4a} $  

Note following points:



* being square $(x+\frac b{2a})^2 $ can only be >= 0 

* when a is positive, $ a\cdot\left(x+\frac b{2a}\right)^2 $ will be always >=0
    
* Base conditions are:  
    *   a is positive AND 
    *   $ ax^2+bx+c $ >= 0 for all values of x. Note: <u><b>"all values of x"</b></u> is important.
  

    
    
For $ ax^2+bx+c >= 0 $ to be true for all (and any) value of x, we must need $ a\cdot\left(x+\frac b{2a}\right)^2-\frac{b^2-4ac}{4a} $ >=0  
    
    
Only $ \frac{b^2-4ac}{4a} $ has the capability to make $ ax^2+bx+c >= 0 $ negative, a already being positive, sign of $ b^2-4ac $ dectates the sign of $ ax^2+bx+c $ i.e. $ a\cdot\left(x+\frac b{2a}\right)^2-\frac{b^2-4ac}{4a} $, when $ \frac{b^2-4ac}{4a} > a\cdot\left(x+\frac b{2a}\right)^2 $ in general.    

    
    
The value of the term $ a\cdot\left(x+\frac b{2a}\right)^2 $ is minimum(0) when    $ x = -\frac{b}{2a} $, in this case $ ax^2+bx+c = a\cdot\left(x+\frac b{2a}\right)^2-\frac{b^2-4ac}{4a} = -\frac{b^2-4ac}{4a} $ ,
    
if $ ax^2+bx+c >=0 $  in this case, following conditions are must (or can be inferred)  
    $ -\frac{b^2-4ac}{4a} >=0 $  
    $ \frac{b^2-4ac}{4a} <= 0 $  
    $ b^2-4ac <=0 $   
    $ b^2-4ac <= 0 $   
    $ b^2 <= 4ac $ 
    
Therefore if a>0 AND $ ax^2+bx+c >= 0 $ for all(any value) of x, including $ x = -\frac{b}{2a} $ , then $ b^2 <= 4ac $ . Note that value of $ b^2-4ac $ is independant of x and therefore $ b^2-4ac <= 0 $ should always be true to have $ ax^2+bx+c >= 0 $ for all values of x. 
    
    


    








